Add lemmas about lookup type and fields to ease working with it
Mostly existentials related to lookup

src/SchemaAux.v
@@ -33,24 +33,87 @@ Section SchemaAux.
     else
       None.
 
+  Lemma get_firstP {A : eqType} (p : pred A) (s : seq A) : reflect (exists2 x, x \in s & p x) (get_first p s).
+  Proof.
+    apply: (iffP idP).
+    - elim: s => // hd tl IH.
+      rewrite /get_first.
+      case: ifP => //.
+        * by exists hd => //; apply mem_head.
+        * by move=> _ /IH; case=> [x Hin Hp]; exists x => //; rewrite in_cons; apply/orP; right.     
+    - case=> x Hin Hp.
+      rewrite /get_first.
+      elim: s Hin => // hd tl IH.
+      rewrite in_cons => /orP [/eqP <- | Htl].
+      by rewrite Hp.
+      case: ifP => // _.
+      by apply: IH.
+  Qed.
+
+  Lemma mem_tail {A : eqType} (tl : seq A) (x hd : A) : x \in tl -> x \in (hd :: tl).
+  Proof.
+      by rewrite in_cons => Hin; apply/orP; right.
+  Qed.
+  
+
+      
+ Lemma get_first_E A (p : pred A) s tdef : (get_first p s = Some tdef) -> get_first p s.
+  Proof.
+    by move=> ->. Qed.
+  
+  (** Checks whether the given type definition has the given name **)
+  Definition has_name (name : @NamedType Name) (tdef : TypeDefinition) : bool :=
+    name == tdef.(tdef_name).
+
+  Lemma has_nameP name tdef : reflect (name = tdef.(tdef_name)) (has_name name tdef).
+  Proof. by apply: (iffP eqP). Qed.
   
   (**
    Looks up a name in the given document, returning the type definition if it
    was declared in the document.
    **)
   Definition lookup_type (ty : NamedType)  : option TypeDefinition :=
-    let n_eq nt tdef := match tdef with
-                       | ScalarTypeDefinition name =>  nt == name 
-                       | ObjectTypeDefinition name _  _ =>  nt == name
-                       | InterfaceTypeDefinition name _ => nt == name
-                       | UnionTypeDefinition name _ => nt == name
-                       | EnumTypeDefinition name _ =>  nt == name
-                       end
-    in
-    get_first (n_eq ty) schema.
+    get_first (has_name ty) schema.
     
 
+  Lemma lookup_typeP ty :
+    reflect (exists2 tdef, tdef \in schema.(type_definitions) & tdef.(tdef_name) = ty)
+            (lookup_type ty).
+  Proof.
+    apply: (iffP idP).
+    - rewrite /lookup_type.
+      move/get_firstP => [x Hin].
+      by rewrite /has_name => /eqP ->; exists x.
+    - case=> tdef Hin <-.
+      rewrite /lookup_type.
+      apply/get_firstP.
+      by exists tdef => //; rewrite /has_name.
+  Qed.
 
+  Lemma lookup_type_isSome ty tdef : lookup_type ty = Some tdef -> lookup_type ty.
+  Proof. by move=> ->. Qed.
+
+
+  Hint Resolve mem_head mem_tail.
+  Lemma lookup_in_schema ty tdef :
+    lookup_type ty = Some tdef ->
+    tdef \in schema.(type_definitions).
+  Proof.
+    rewrite /lookup_type.
+    elim: (schema.(type_definitions)) => // hd tl IH.
+    rewrite /get_first.
+    by case: has_name => //; [case=> -> | move/IH => //; apply: mem_tail].
+  Qed.
+
+  Lemma lookup_type_name ty tdef : lookup_type ty = Some tdef -> ty = tdef.(tdef_name).
+  Proof.
+    rewrite /lookup_type.
+    elim: schema.(type_definitions) => // hd tl IH.
+    rewrite /get_first.
+      by case Hn : has_name => //; move/has_nameP: Hn => ->; case => ->.
+  Qed.
+
+  
   (** Checks whether the given type is defined as a Scalar in the Schema **)
   Definition is_scalar_type (ty : NamedType) : bool :=
     match (lookup_type ty) with
@@ -58,6 +121,8 @@ Section SchemaAux.
     | _ => false
     end.
 
+
+      
   (** Checks whether the given type is defined as an Object in the Schema **)
   Equations is_object_type (ty : @NamedType Name) : bool :=
     is_object_type ty with (lookup_type ty) =>
@@ -151,6 +216,17 @@ Section SchemaAux.
 
   (** Check whether a given name is declared in the schema, as a type definition **)
   Definition is_declared (name : Name) : bool := name \in schema_names.
+
+
+  (** Checks whether the field has the given name **)
+  Definition has_field_name (fname : Name) (fld : FieldDefinition) :=
+    fname == fld.(field_name).
+
+  Lemma has_field_nameP (fname : Name) (fld : FieldDefinition) :
+    reflect (fname = fld.(field_name)) (has_field_name fname fld).
+  Proof.
+    by apply: (iffP eqP). Qed.
+    
   
   (**
      Gets the first field definition from a given type that matches the given field name. 
@@ -158,10 +234,27 @@ Section SchemaAux.
    **)
   Definition lookup_field_in_type (ty : NamedType) (fname : Name) : option FieldDefinition :=
     if lookup_type ty is Some tdef then
-      get_first (fun fld => fld.(field_name) == fname) tdef.(tdef_fields)
+      get_first (has_field_name fname) tdef.(tdef_fields)
     else
       None.
 
+
+  Lemma lookup_field_in_typeP ty fname :
+    reflect (exists tdef fld, [/\ lookup_type ty = Some tdef,
+                          fld \in tdef.(tdef_fields) &
+                                  fld.(field_name) = fname]) (lookup_field_in_type ty fname).
+  Proof.
+    apply: (iffP idP).
+    - rewrite /lookup_field_in_type.
+      case Hlook: lookup_type => [tdef|] //.
+      move/get_firstP=> [fld Hin /has_field_nameP ->].
+      by exists tdef, fld.
+    - case=> [tdef [fld [Hlook Hin <-]]].
+      rewrite /lookup_field_in_type Hlook /=.
+      apply/get_firstP.
+      by exists fld => //; rewrite /has_field_name.
+  Qed.
+  
   (** 
       Gets the type of the first field definition from a given type that matches the given field name. 
       If the type is not declared in the Schema or the field does not belong to the type, then it returns None.
@@ -169,11 +262,23 @@ Section SchemaAux.
    **)
   Definition lookup_field_type (ty : NamedType) (fname : Name)  : option type :=
     match lookup_field_in_type ty fname with
-    | Some fieldDef => Some (return_type fieldDef) 
+    | Some fld => Some fld.(return_type)
     | None => None
     end.
 
 
+  Lemma lookup_field_typeP ty ty' fname :
+    reflect (exists2 fld, lookup_field_in_type ty fname = Some fld & fld.(return_type) = ty')
+            (lookup_field_type ty fname == Some ty').
+  Proof.
+    apply: (iffP eqP).
+    - rewrite /lookup_field_type.
+      case lookup_field_in_type => // fld.
+      by case=> <-; exists fld.
+    - move=> [fld Hlook <-].
+      by rewrite /lookup_field_type Hlook.
+  Qed.
+      
     (**
      Get the union's types' names.
      If the type is not declared as Union in the Schema, then returns None.
@@ -184,7 +289,18 @@ Section SchemaAux.
     | _ => fset0
     end.
 
+  (* Valid for wf schema *)
+  Lemma union_members_nfset0P ty : reflect (is_union_type ty) (union_members ty != fset0).
+  Proof.
+    apply: (iffP idP).
+    - move/fset0Pn=> [x].
+      rewrite /union_members.
+      funelim (is_union_type ty) => //; rewrite Heq //.
+    - funelim (is_union_type ty) => // _.
+      rewrite /union_members Heq.
+  Admitted.
 
+      
   (**
      Checks whether the given type declares implementation of another type.
    **)
@@ -195,9 +311,37 @@ Section SchemaAux.
     end.
 
 
+  
+  Lemma in_intfs ty (tdef : @TypeDefinition Name):
+    ty \in tdef_intfs tdef ->
+           exists n flds, tdef = ObjectTypeDefinition n (tdef_intfs tdef) flds.
+  Proof.
+    rewrite /tdef_intfs.
+    case: tdef => // o i flds Hin.
+    by exists o, flds.
+  Qed.
+  
+  Lemma declares_implementationP ty ity :
+    reflect (exists2 tdef, lookup_type ty = Some tdef & ity \in tdef_intfs tdef)
+            (declares_implementation ty ity).
+  Proof.
+    apply: (iffP idP).
+    - rewrite /declares_implementation.
+      case Hlook : lookup_type => [tdef|] //.
+        by exists tdef => // {Hlook}; case: tdef H => //.
+    - move=> [tdef Hlook Hin].
+      rewrite /declares_implementation Hlook.
+      by move: (in_intfs Hin) => [n [flds ->]].
+  Qed.
+  
   Definition implements_interface (iname : NamedType) (tdef : @TypeDefinition Name) : bool :=
     iname \in tdef.(tdef_intfs).
-  
+
+
+
+
+
+    
   (**
      Gets the first argument definition that matches the given argument name, from the
      given type and field. If the argument is not defined then it returns None.
@@ -230,14 +374,55 @@ Section SchemaAux.
     | _ => fset0
     end.
   
-  Definition implementation (ty : NamedType) : seq NamedType :=
-    match lookup_type ty with
-    | Some (InterfaceTypeDefinition iname _) =>
-      let filtered := [seq tdef <- schema | implements_interface iname tdef]
-      in
-      fset [seq tdef.(tdef_name) | tdef <- filtered]
-    | _ => [::]
-    end.
+  Definition implementation (ty : NamedType) : {fset NamedType} :=
+    fset [seq tdef.(tdef_name) | tdef <- schema & implements_interface ty tdef].
+
+
+
+  Lemma seq0Pn (A : eqType) (s : seq A) : reflect (exists x, x \in s) (s != [::]).
+  Proof.
+    apply: (iffP idP) => //.
+    - by case: s => // hd tl _; exists hd; apply: mem_head.
+    - by case: s => //; case=> [x]; rewrite in_nil.
+  Qed.
+  
+  Lemma fset_N_fset0 (A : ordType) (s : seq A) :
+    fset s != fset0 <->
+    s != [::].
+  Proof. split.
+    - by case: s => //; move/fset0Pn=> [x]; rewrite in_fset.
+    - by move/seq0Pn=> [x Hin]; apply/fset0Pn; exists x; rewrite in_fset.
+  Qed.
+
+
+  Lemma in_N_nilP {A : eqType} (s : seq A) : reflect (exists x, x \in s) (s != [::]).
+  Proof.
+    apply: (iffP idP) => //.
+    by case: s => // a *; exists a; rewrite inE; apply/orP; left. 
+    by case: s => //; case=> [x]; rewrite in_nil.
+  Qed.
+
+  Lemma implementationP ty :
+    reflect (exists2 x, x \in schema.(type_definitions) & implements_interface ty x) (implementation ty != fset0).
+  Proof.
+    apply: (iffP idP).
+    - rewrite /implementation.
+      move/fset_N_fset0/in_N_nilP => [x /mapP [x']].
+      by rewrite mem_filter => /andP [Himpl Hin] _; exists x'.
+    - case=> [x Hin Himpl].
+      rewrite /implementation fset_N_fset0.
+      apply/seq0Pn. exists (x.(tdef_name)).
+      by apply/mapP; exists x => //;rewrite mem_filter; apply/andP.
+  Qed.
+      
+  Lemma implementation_has ty :
+    implementation ty != fset0 <-> has (implements_interface ty) schema.
+  Proof.
+    split.
+    - by move/implementationP=> H; apply/hasP.
+    - by move/hasP=> H; apply/implementationP.
+  Qed.
+    
 
   Lemma declares_in_implementation t ty :
     (declares_implementation t ty) <-> (t \in implementation ty).
